Lp2lc/Active/STLC/Proof.lean
@@ -40,51 +40,51 @@ The definition is designed to talk about "(x : T)"-like assumptions.
 open List
 
 lemma context_terms_iff_in_list (x : Var) (Γ : Env) :
-    (x ∈ context_terms Γ) ↔ in_context x Γ := by
+    (x ∈ Env.context_terms Γ) ↔ Env.in_context x Γ := by
   induction Γ
   case nil =>
-    simp only [context_terms, Finset.notMem_empty, in_context]
+    simp only [Env.context_terms, Finset.notMem_empty, Env.in_context]
   case cons b Γ' f =>
-    simp only [context_terms, Finset.mem_union, Finset.mem_singleton, in_context]
+    simp only [Env.context_terms, Finset.mem_union, Finset.mem_singleton, Env.in_context]
     rw [f]
 
 lemma not_context_terms_to_not_in_context x Γ :
-    ¬ (x ∈ context_terms Γ) →  ¬ in_context x Γ := by
+    ¬ (x ∈ Env.context_terms Γ) →  ¬ Env.in_context x Γ := by
   rw [context_terms_iff_in_list]
   simp
 
 lemma in_context_append_neg (x : Var) (Γ Δ : Env) :
-    ¬ (in_context x (Γ ++ Δ)) → ¬ (in_context x Γ) ∧ ¬ (in_context x Δ) := by
+    ¬ (Env.in_context x (Γ ++ Δ)) → ¬ (Env.in_context x Γ) ∧ ¬ (Env.in_context x Δ) := by
   intro H
   induction Γ
   case nil =>
-    simp only [in_context, not_false_eq_true, true_and] at H ⊢
+    simp only [Env.in_context, not_false_eq_true, true_and] at H ⊢
     rwa [nil_append] at H
   case cons b Γ' f =>
-    simp [in_context] at H f ⊢
+    simp [Env.in_context] at H f ⊢
     exact ⟨⟨H.1, (f (H.2)).1⟩, (f (H.2)).2⟩
 
 lemma in_context_append_neg' (x : Var) (Γ Δ : Env) :
-    ¬ (in_context x Γ) ∧ ¬ (in_context x Δ) → ¬ (in_context x (Γ ++ Δ)) := by
+    ¬ (Env.in_context x Γ) ∧ ¬ (Env.in_context x Δ) → ¬ (Env.in_context x (Γ ++ Δ)) := by
   rintro ⟨H1, H2⟩
   induction Γ
   case nil =>
     simp only [nil_append]
     exact H2
   case cons b Γ' f =>
-    simp [in_context, append_eq] at H1 ⊢
+    simp [Env.in_context, append_eq] at H1 ⊢
     exact ⟨H1.1, f H1.2⟩
 
 -- We can only bind variable once per Env --
 
 --Properties of valid contexts
 lemma valid_push (Γ : Env) (x : Var) (T : Typ) :
-    valid_ctx Γ → ¬ (in_context x Γ) → valid_ctx ((([(x, Bind.bind_typ T)] : Env) ++ Γ)) := by
+    Env.valid_ctx Γ → ¬ (Env.in_context x Γ) → Env.valid_ctx ((([(x, Bind.bind_typ T)] : Env) ++ Γ)) := by
   simp only [singleton_append]
-  exact (valid_ctx.valid_cons Γ x T)
+  exact (Env.valid_ctx.valid_cons Γ x T)
 
 lemma valid_remove_mid (Γ Δ Ψ : Env) :
-    valid_ctx (Ψ ++ Δ ++ Γ) -> valid_ctx (Ψ ++ Γ) := by
+    Env.valid_ctx (Ψ ++ Δ ++ Γ) -> Env.valid_ctx (Ψ ++ Γ) := by
   induction Ψ
   case nil =>
     induction Δ
@@ -102,7 +102,7 @@ lemma valid_remove_mid (Γ Δ Ψ : Env) :
     cases H
     next x S p p' =>
       simp only [cons_append, append_assoc] at f p ⊢
-      apply valid_ctx.valid_cons
+      apply Env.valid_ctx.valid_cons
       exact (f p)
       apply in_context_append_neg'
       constructor
@@ -110,16 +110,16 @@ lemma valid_remove_mid (Γ Δ Ψ : Env) :
       exact (in_context_append_neg _ _ _ (in_context_append_neg _ _ _ p').2).2
 
 lemma valid_remove_mid_cons (x : Var) (T : Typ) (Γ Δ : Env) :
-    valid_ctx (Δ ++ (x, Bind.bind_typ T ) :: Γ)
-    → valid_ctx (Δ ++ Γ) := by
+    Env.valid_ctx (Δ ++ (x, Bind.bind_typ T ) :: Γ)
+    → Env.valid_ctx (Δ ++ Γ) := by
   intro H
   simp only [append_cons Δ (x, Bind.bind_typ T ) Γ] at H
   apply valid_remove_mid
   exact H
 
 lemma valid_remove_cons (x : Var) (T : Typ) (Γ : Env) :
-    valid_ctx ((x, Bind.bind_typ T ) :: Γ)
-    → valid_ctx (Γ) := by
+    Env.valid_ctx ((x, Bind.bind_typ T ) :: Γ)
+    → Env.valid_ctx (Γ) := by
   intro H
   rw [← nil_append Γ]
   apply valid_remove_mid_cons
@@ -127,52 +127,52 @@ lemma valid_remove_cons (x : Var) (T : Typ) (Γ : Env) :
   exact H
 
 --Extracting (x : T) from a Env
-lemma binds_singleton (x : Var) (T : Typ) : binds x T (([(x, Bind.bind_typ T)] : Env)) := by
-  simp only [binds]
-  simp only [get]
+lemma binds_singleton (x : Var) (T : Typ) : Env.binds x T (([(x, Bind.bind_typ T)] : Env)) := by
+  simp only [Env.binds]
+  simp only [Env.get]
   simp only [ite_true, Bind.unbox_typ]
 
 lemma binds_singleton_tail (x : Var) (T : Typ) (Γ : Env) :
-    binds x T ((([(x, Bind.bind_typ T)] : Env) ++ Γ)) := by
-  simp [binds, get, append_eq, nil_append, ite_true]
+    Env.binds x T ((([(x, Bind.bind_typ T)] : Env) ++ Γ)) := by
+  simp [Env.binds, Env.get, append_eq, nil_append, ite_true]
 
 lemma binds_tail (x : Var) (T : Typ) (Γ Δ : Env) :
-    binds x T Γ → (¬ (in_context x Δ)) → binds x T (Δ ++ Γ) := by
+    Env.binds x T Γ → (¬ (Env.in_context x Δ)) → Env.binds x T (Δ ++ Γ) := by
   intro bx nx
-  simp [binds] at bx ⊢
+  simp [Env.binds] at bx ⊢
   induction Δ
   case nil =>
     simp only [nil_append, bx]
   case cons b Δ' f' =>
-    simp [in_context] at nx
+    simp [Env.in_context] at nx
     push_neg at nx
-    simp [get, append_eq]
+    simp [Env.get, append_eq]
     rw [if_neg nx.1]
     apply (f' nx.2)
 
 lemma binds_head (x : Var) (T : Typ) (Γ Δ : Env) :
-    binds x T Γ → binds x T (Γ ++ Δ) := by
+    Env.binds x T Γ → Env.binds x T (Γ ++ Δ) := by
   induction Γ
   case nil =>
     simp
   case cons b Γ' f =>
-    simp only [binds, get, append_eq]
+    simp only [Env.binds, Env.get, append_eq]
     by_cases hxb : x = b.1
-    . simp only [cons_append, get]
+    . simp only [cons_append, Env.get]
       rw [if_pos hxb, if_pos hxb]
       exact id
-    . simp only [cons_append, get]
+    . simp only [cons_append, Env.get]
       rw [if_neg hxb]
       intro H
-      simp [binds] at f
+      simp [Env.binds] at f
       rw [if_neg hxb]
       exact (f H)
 
---Case analysis on binds
+--Case analysis on Env.binds
 lemma binds_concat_inv' (x : Var) (T : Typ) (Γ Δ : Env) :
-    binds x T (Γ ++ Δ)
-    → ((in_context x Γ) ∨ ¬(binds x T Δ))
-    → (binds x T Γ) := by
+    Env.binds x T (Γ ++ Δ)
+    → ((Env.in_context x Γ) ∨ ¬(Env.binds x T Δ))
+    → (Env.binds x T Γ) := by
   induction Γ
   case nil =>
     simp
@@ -185,10 +185,10 @@ lemma binds_concat_inv' (x : Var) (T : Typ) (Γ Δ : Env) :
       . simp [if_neg hxb] at bxT ⊢
         apply f
         exact bxT
-        simp [in_context, hxb] at h1
+        simp [Env.in_context, hxb] at h1
         left
         exact h1
-    . simp only [binds, get]
+    . simp only [Env.binds, Env.get]
       by_cases hxb : x = b.1
       . simp [if_pos hxb] at bxT ⊢
         exact bxT
@@ -199,8 +199,8 @@ lemma binds_concat_inv' (x : Var) (T : Typ) (Γ Δ : Env) :
         exact h2
 
 lemma binds_concat_inv (x : Var) (T : Typ) (Γ Δ : Env) :
-    binds x T (Γ ++ Δ)
-    → ((¬ (in_context x Γ)) ∧ (binds x T Δ)) ∨ (binds x T Γ) := by
+    Env.binds x T (Γ ++ Δ)
+    → ((¬ (Env.in_context x Γ)) ∧ (Env.binds x T Δ)) ∨ (Env.binds x T Γ) := by
   intro bxT
   refine Iff.mpr or_iff_not_imp_left ?_
   intro H
@@ -209,8 +209,8 @@ lemma binds_concat_inv (x : Var) (T : Typ) (Γ Δ : Env) :
   exact Iff.mpr or_iff_not_imp_left H
 
 lemma binds_singleton_inv (x y : Var) (X Y : Typ) :
-    binds x X (([(y, Bind.bind_typ Y)] : Env)) → (x = y) ∧ (X = Y) := by
-  simp only [binds, get]
+    Env.binds x X (([(y, Bind.bind_typ Y)] : Env)) → (x = y) ∧ (X = Y) := by
+  simp only [Env.binds, Env.get]
   intro H
   by_cases hxy : x = y
   . simp [if_pos hxy] at H
@@ -218,16 +218,16 @@ lemma binds_singleton_inv (x y : Var) (X Y : Typ) :
   . simp [if_neg hxy] at H
 
 lemma binds_mid (x : Var) (T : Typ) (Δ Γ : Env) :
-    valid_ctx (Γ ++ (([(x, Bind.bind_typ T)] : Env)) ++ Δ)
-    → binds x T (Γ ++ (([(x, Bind.bind_typ T)] : Env)) ++ Δ) := by
+    Env.valid_ctx (Γ ++ (([(x, Bind.bind_typ T)] : Env)) ++ Δ)
+    → Env.binds x T (Γ ++ (([(x, Bind.bind_typ T)] : Env)) ++ Δ) := by
   induction Γ
   case nil =>
-    simp only [nil_append, singleton_append, binds, get, append_eq, ite_true, implies_true, Bind.unbox_typ]
+    simp only [nil_append, singleton_append, Env.binds, Env.get, append_eq, ite_true, implies_true, Bind.unbox_typ]
   case cons b Γ' f =>
     intro H
     cases H
     next y S H' g =>
-      simp only [binds, get, append_eq, append_assoc, singleton_append] at f H' g ⊢
+      simp only [Env.binds, Env.get, append_eq, append_assoc, singleton_append] at f H' g ⊢
       by_cases hxy : x = y
       . simp [if_pos hxy]
         have ⟨_, t2⟩ := in_context_append_neg _ _ _ g
@@ -239,17 +239,17 @@ lemma binds_mid (x : Var) (T : Typ) (Δ Γ : Env) :
         exact (f H')
 
 lemma binds_mid_eq (x : Var) (T S : Typ) (Γ Δ : Env) :
-    binds x T (Δ ++ (([(x, Bind.bind_typ S)] : Env)) ++ Γ)
-    → valid_ctx (Δ ++ (([(x, Bind.bind_typ S)] : Env)) ++ Γ) →  T = S := by
+    Env.binds x T (Δ ++ (([(x, Bind.bind_typ S)] : Env)) ++ Γ)
+    → Env.valid_ctx (Δ ++ (([(x, Bind.bind_typ S)] : Env)) ++ Γ) →  T = S := by
   induction Δ
   case nil =>
-    simp only [binds, get, append_eq, nil_append, ite_true, Option.some.injEq, singleton_append]
+    simp only [Env.binds, Env.get, append_eq, nil_append, ite_true, Option.some.injEq, singleton_append]
     exact (fun p _ => p.symm)
   case cons b Δ' f =>
     intro p H
     cases H
     next y S' H' g =>
-      simp only [binds, get, append_eq, append_assoc, singleton_append] at p f H' g ⊢
+      simp only [Env.binds, Env.get, append_eq, append_assoc, singleton_append] at p f H' g ⊢
       by_cases hxy : x = y
       . have ⟨_, t2⟩ := in_context_append_neg _ _ _ g
         simp at t2
@@ -260,20 +260,20 @@ lemma binds_mid_eq (x : Var) (T S : Typ) (Γ Δ : Env) :
         exact (f p H')
 
 lemma binds_mid_eq_cons (x : Var) (T S : Typ) (Γ Δ : Env) :
-    binds x T (Δ ++ (x, Bind.bind_typ S ) :: Γ)
-    → valid_ctx (Δ ++ (x, Bind.bind_typ S ) :: Γ) → T = S := by
+    Env.binds x T (Δ ++ (x, Bind.bind_typ S ) :: Γ)
+    → Env.valid_ctx (Δ ++ (x, Bind.bind_typ S ) :: Γ) → T = S := by
   intro p H
   simp only [append_cons Δ (x, Bind.bind_typ S ) Γ] at p H
   exact (binds_mid_eq x T S Γ Δ p H)
 
---Additional properties of binds
+--Additional properties of Env.binds
 lemma binds_in_context (x : Var) (T : Typ) (Γ : Env) :
-    binds x T Γ → in_context x Γ := by
+    Env.binds x T Γ → Env.in_context x Γ := by
   induction Γ
   case nil =>
     simp
   case cons b Γ' f =>
-    simp only [binds, get, in_context] at f ⊢
+    simp only [Env.binds, Env.get, Env.in_context] at f ⊢
     by_cases hxb : x = b.1
     . simp only [if_pos hxb]
       intro _
@@ -283,21 +283,21 @@ lemma binds_in_context (x : Var) (T : Typ) (Γ : Env) :
       exact (Or.inr (f p))
 
 lemma binds_fresh (x : Var) (T : Typ) (Γ : Env) :
-    ¬ in_context x Γ → ¬ binds x T Γ := by
+    ¬ Env.in_context x Γ → ¬ Env.binds x T Γ := by
   intro hxin hb
   exact hxin (binds_in_context x T Γ hb)
 
 lemma binds_concat_ok (x : Var) (T : Typ) (Γ Δ : Env) :
-    binds x T Γ -> valid_ctx (Δ ++ Γ) -> binds x T (Δ ++ Γ) := by
+    Env.binds x T Γ -> Env.valid_ctx (Δ ++ Γ) -> Env.binds x T (Δ ++ Γ) := by
   induction Δ
   case nil =>
-    simp only [binds, nil_append]
+    simp only [Env.binds, nil_append]
     exact (fun p _ => p)
   case cons b Δ' f =>
     intro p H
     cases H
     next y S H' g =>
-      simp only [binds, get, append_eq] at H' ⊢
+      simp only [Env.binds, Env.get, append_eq] at H' ⊢
       by_cases hxy : x = y
       . simp [if_pos hxy]
         by_contra
@@ -309,18 +309,18 @@ lemma binds_concat_ok (x : Var) (T : Typ) (Γ Δ : Env) :
         exact (f p H')
 
 lemma binds_weaken (x : Var) (T : Typ) (Γ Δ Ψ: Env) :
-    binds x T (Ψ ++ Γ)
-    → valid_ctx (Ψ ++ Δ ++ Γ)
-    → binds x T (Ψ ++ Δ ++ Γ) := by
+    Env.binds x T (Ψ ++ Γ)
+    → Env.valid_ctx (Ψ ++ Δ ++ Γ)
+    → Env.binds x T (Ψ ++ Δ ++ Γ) := by
   induction Ψ
   case nil =>
-    simp only [binds, nil_append]
+    simp only [Env.binds, nil_append]
     exact (fun p H => (binds_concat_ok _ _ _ _ p H))
   case cons b Ψ' f =>
     intro p H
     cases H
     next y S H' g =>
-      simp only [binds, get, append_eq, append_assoc, in_context] at f H' p g ⊢
+      simp only [Env.binds, Env.get, append_eq, append_assoc, Env.in_context] at f H' p g ⊢
       by_cases hxy : x = y
       . simp [if_pos hxy] at p ⊢
         exact p
@@ -328,12 +328,12 @@ lemma binds_weaken (x : Var) (T : Typ) (Γ Δ Ψ: Env) :
         exact (f p H')
 
 lemma binds_weaken_at_head (x : Var) (T : Typ) (Γ Δ : Env) :
-    binds x T Δ → valid_ctx (Γ ++ Δ)
-    → binds x T (Γ ++ Δ) := (binds_weaken x T Δ Γ [])
+    Env.binds x T Δ → Env.valid_ctx (Γ ++ Δ)
+    → Env.binds x T (Γ ++ Δ) := (binds_weaken x T Δ Γ [])
 
 lemma binds_remove_mid (x y : Var) (T S : Typ) (Γ Δ : Env) :
-    binds x T (Γ ++ ((([(y, Bind.bind_typ S)] : Env)) ++ Δ))
-    → x ≠ y → binds x T (Γ ++ Δ) := by
+    Env.binds x T (Γ ++ ((([(y, Bind.bind_typ S)] : Env)) ++ Δ))
+    → x ≠ y → Env.binds x T (Γ ++ Δ) := by
   intro p H
   have t := (binds_concat_inv x T Γ ((([(y, Bind.bind_typ S)] : Env)) ++ Δ) p)
   rcases t with ⟨t11, t12⟩ | t2
@@ -344,8 +344,8 @@ lemma binds_remove_mid (x y : Var) (T S : Typ) (Γ Δ : Env) :
   . apply (binds_head _ _ _ _ t2)
 
 lemma binds_remove_mid_cons  (x y : Var) (T S : Typ) (Γ Δ : Env) :
-    binds x T (Δ ++ (y, Bind.bind_typ S ) :: Γ)
-    → x ≠ y → binds x T (Δ ++ Γ) := by
+    Env.binds x T (Δ ++ (y, Bind.bind_typ S ) :: Γ)
+    → x ≠ y → Env.binds x T (Δ ++ Γ) := by
   intro H p
   apply (binds_remove_mid x y T S Δ Γ)
   rwa [append_cons, append_assoc] at H
@@ -1353,7 +1353,7 @@ lemma multi_red_iff_multi_para : ∀ t1 t2, (multi_red t1 t2) ↔ (multi_para t1
 open typing
 
 --Typing judgments only allow valid contexts.
-lemma typing_valid_ctx  Γ t T : typing Γ t T → valid_ctx Γ := by
+lemma typing_valid_ctx  Γ t T : typing Γ t T → Env.valid_ctx Γ := by
   intro H
   induction H
   case typ_var _ _ _ h _ =>
@@ -1370,7 +1370,7 @@ lemma typing_valid_ctx  Γ t T : typing Γ t T → valid_ctx Γ := by
 --Weakining Rule
 lemma typing_weakening_strengthened' (Γ Δ Ψ' : Env) (t : Trm) (T : Typ) :
     typing Ψ' t T → (Ψ : Env) → Ψ' = Ψ ++ Γ
-    → valid_ctx (Ψ ++ Δ ++ Γ)
+    → Env.valid_ctx (Ψ ++ Δ ++ Γ)
     → typing (Ψ ++ Δ ++ Γ) t T := by
   intro H
   induction H
@@ -1382,12 +1382,12 @@ lemma typing_weakening_strengthened' (Γ Δ Ψ' : Env) (t : Trm) (T : Typ) :
     exact (binds_weaken _ _ _ _ _ fT' f)
   case typ_abs L φ' s T1 T2 _ fT2 =>
     intro φ p f
-    apply typ_abs (L ∪ context_terms (φ ++ Δ ++ Γ))
+    apply typ_abs (L ∪ Env.context_terms (φ ++ Δ ++ Γ))
     intro x hx
     simp at hx
     apply (fT2 x hx.1 ((x, Bind.bind_typ T1) :: φ))
     simp [p]
-    apply valid_ctx.valid_cons
+    apply Env.valid_ctx.valid_cons
     exact f
     simp [append_cons]
     intro q
@@ -1400,7 +1400,7 @@ lemma typing_weakening_strengthened' (Γ Δ Ψ' : Env) (t : Trm) (T : Typ) :
 
 lemma typing_weakening_strengthened (Γ Δ Ψ : Env) (t : Trm) (T : Typ) :
     typing (Ψ ++ Γ) t T
-    → valid_ctx (Ψ ++ Δ ++ Γ)
+    → Env.valid_ctx (Ψ ++ Δ ++ Γ)
     → typing (Ψ ++ Δ ++ Γ) t T := by
   intro H p
   apply (typing_weakening_strengthened' _ _ (Ψ ++ Γ))
@@ -1409,7 +1409,7 @@ lemma typing_weakening_strengthened (Γ Δ Ψ : Env) (t : Trm) (T : Typ) :
   exact p
 
 lemma typing_weakening (Γ Δ : Env) (t : Trm) (T : Typ) :
-    typing (Γ) t T → valid_ctx (Δ ++ Γ)
+    typing (Γ) t T → Env.valid_ctx (Δ ++ Γ)
     → typing (Δ ++ Γ) t T := by
   intro H p
   rw [← nil_append (Δ ++ Γ)] at p
@@ -1419,7 +1419,7 @@ lemma typing_weakening (Γ Δ : Env) (t : Trm) (T : Typ) :
   exact p
 
 lemma typing_weakening_head (Γ : Env) (t : Trm) (T S : Typ) (x : Var):
-    ¬ (in_context x Γ) → typing Γ t T
+    ¬ (Env.in_context x Γ) → typing Γ t T
     → typing ((x, Bind.bind_typ S ) :: Γ) t T := by
   intro notxl typt
   rw [← nil_append ((x, Bind.bind_typ S ) :: Γ), append_cons, nil_append]
@@ -1430,8 +1430,8 @@ lemma typing_weakening_head (Γ : Env) (t : Trm) (T S : Typ) (x : Var):
 
 --Substitution Rule
 lemma typing_subst_var_case (Γ Δ : Env) (u : Trm) (S T : Typ) (z x : Var) :
-    binds x T (Δ ++ (z, Bind.bind_typ S ) :: Γ)
-    → valid_ctx (Δ ++ (z, Bind.bind_typ S ) :: Γ)
+    Env.binds x T (Δ ++ (z, Bind.bind_typ S ) :: Γ)
+    → Env.valid_ctx (Δ ++ (z, Bind.bind_typ S ) :: Γ)
     → typing Γ u S → typing (Δ ++ Γ) ([z // u] ($ x)) T := by
   intro b v t
   simp only [subst]
@@ -1487,7 +1487,7 @@ lemma typing_subst_strengthened' Γ Δ' t u S T z :
   case typ_abs L ψ s S1 S2 h h' =>
     intro Δ p _ f
     simp only [subst]
-    apply typ_abs (L ∪ context_terms (Δ ++ Γ) ∪ {z}) (Δ ++ Γ) ([z // u] s) S1 S2
+    apply typ_abs (L ∪ Env.context_terms (Δ ++ Γ) ∪ {z}) (Δ ++ Γ) ([z // u] s) S1 S2
     intro x hx
     have hxz : x ≠ z := by
       intro q
@@ -1539,14 +1539,14 @@ lemma typing_subst (Γ : Env) (t u : Trm) (S T : Typ) (z : Var) :
 --------------------------------------------
 
 lemma typing_rename (Γ : Env) (x y : Var) (t : Trm) (T1 T2 : Typ) :
-    x ∉ fv t →  ¬ (in_context x Γ)
-    → y ∉ fv t →  ¬ (in_context y Γ)
+    x ∉ fv t →  ¬ (Env.in_context x Γ)
+    → y ∉ fv t →  ¬ (Env.in_context y Γ)
     → typing ((x, Bind.bind_typ T1) :: Γ) (open₀ t ($ x)) T2
     → typing ((y, Bind.bind_typ T1) :: Γ) (open₀ t ($ y)) T2 := by
   intro hx fx _ fy R
   by_cases hxy : x = y
   . rwa [hxy] at R
-  . have ok_ctx : valid_ctx Γ := by
+  . have ok_ctx : Env.valid_ctx Γ := by
       apply valid_remove_cons
       apply typing_valid_ctx
       exact R
@@ -1567,11 +1567,11 @@ lemma typing_rename (Γ : Env) (x y : Var) (t : Trm) (T1 T2 : Typ) :
     simp
 
 lemma typing_abs_intro (Γ : Env) (x : Var) (t : Trm) (T1 T2 : Typ) :
-    x ∉ fv t →  ¬ (in_context x Γ)
+    x ∉ fv t →  ¬ (Env.in_context x Γ)
     → typing ((x, Bind.bind_typ T1) :: Γ) (open₀ t ($ x)) T2
     → typing Γ (abs T1 t) (T1 -> T2) := by
   intro hx fx R
-  apply typ_abs (fv t ∪ context_terms Γ)
+  apply typ_abs (fv t ∪ Env.context_terms Γ)
   intro y hy
   simp at hy
   apply (typing_rename _ _ _ _ _ _ hx fx)
@@ -1897,18 +1897,18 @@ def multi_subst (L : Finset Var) (f : L → Trm) : Trm → Trm
 
 --context_type takes a term in a Env and outputs its type
 @[simp]
-def context_type Γ (x : context_terms Γ) : Typ :=
+def context_type Γ (x : Env.context_terms Γ) : Typ :=
   match Γ, x with
-  | [], ⟨_, h⟩ => by simp [context_terms] at h
+  | [], ⟨_, h⟩ => by simp [Env.context_terms] at h
   | (x, Bind.bind_typ T) :: Γ, ⟨x', h⟩ =>
     if ha : x' = x then
       T
     else
-      context_type Γ ⟨x', by simpa [context_terms, ha] using h⟩
+      context_type Γ ⟨x', by simpa [Env.context_terms, ha] using h⟩
 
 --substitution over the empty Env does nothing
-lemma multi_subst_over_emp t (f : context_terms [] → Trm) :
-    (multi_subst (context_terms []) f t) = t := by
+lemma multi_subst_over_emp t (f : Env.context_terms [] → Trm) :
+    (multi_subst (Env.context_terms []) f t) = t := by
   induction t
   case bvar i =>
     simp
@@ -1923,8 +1923,8 @@ lemma multi_subst_over_emp t (f : context_terms [] → Trm) :
 
 --substitution over [(x,T)] is the same as usual (single) substitution
 lemma multi_subst_at_singleton t x T :
-    (f : context_terms (([(x, Bind.bind_typ T)] : Env)) → Trm)
-    → (multi_subst (context_terms (([(x, Bind.bind_typ T)] : Env))) f t)
+    (f : Env.context_terms (([(x, Bind.bind_typ T)] : Env)) → Trm)
+    → (multi_subst (Env.context_terms (([(x, Bind.bind_typ T)] : Env))) f t)
       = ([x // (f ⟨x, by simp⟩)] t) := by
   intro f
   induction t
@@ -1945,8 +1945,8 @@ lemma multi_subst_at_singleton t x T :
 --if we have a function of terms of a Env, say f,
 --for a term u and variable x, we can extend the f with mapping x → u
 @[simp]
-def add_term Γ (f : context_terms Γ → Trm)
-    (u : Trm) y T (x : context_terms ((y, Bind.bind_typ T) :: Γ)) : Trm := by
+def add_term Γ (f : Env.context_terms Γ → Trm)
+    (u : Trm) y T (x : Env.context_terms ((y, Bind.bind_typ T) :: Γ)) : Trm := by
   rcases x with ⟨x' , h⟩
   by_cases p : x' = y
   . exact u
@@ -1955,15 +1955,15 @@ def add_term Γ (f : context_terms Γ → Trm)
 
 --If y does not appear in t, then substitution over a Env (y,T) ++ Γ
 --is the same as substitution over Γ
-lemma multi_subst_fresh Γ t u y T (h : y ∉ (fv t)) (f : context_terms Γ → Trm) :
-    (multi_subst (context_terms ((y, Bind.bind_typ T) :: Γ)) (add_term Γ f u y T) t)
-     = (multi_subst (context_terms Γ) f t) := by
+lemma multi_subst_fresh Γ t u y T (h : y ∉ (fv t)) (f : Env.context_terms Γ → Trm) :
+    (multi_subst (Env.context_terms ((y, Bind.bind_typ T) :: Γ)) (add_term Γ f u y T) t)
+     = (multi_subst (Env.context_terms Γ) f t) := by
   induction t
   case bvar i =>
     rfl
   case fvar x =>
     simp [fv] at h
-    simp only [multi_subst, context_terms, Finset.mem_union, Finset.mem_singleton, add_term]
+    simp only [multi_subst, Env.context_terms, Finset.mem_union, Finset.mem_singleton, add_term]
     have p : x ≠ y := fun q => h q.symm
     simp [p]
   case abs T u hu =>
@@ -1978,10 +1978,10 @@ lemma multi_subst_fresh Γ t u y T (h : y ∉ (fv t)) (f : context_terms Γ → 
 
 
 --substitution over a Env distributes over opening
-lemma multi_subst_open_lemma_1 t1 t2 Γ : (f : context_terms Γ → Trm)
-   → (∀ x (h : x ∈ context_terms Γ), lc (f ⟨x,h⟩)) → (j : ℕ)
-   → (multi_subst (context_terms Γ) f ({j ~> t2} t1))
-     = ({j ~> multi_subst (context_terms Γ) f t2} (multi_subst (context_terms Γ) f t1)) := by
+lemma multi_subst_open_lemma_1 t1 t2 Γ : (f : Env.context_terms Γ → Trm)
+   → (∀ x (h : x ∈ Env.context_terms Γ), lc (f ⟨x,h⟩)) → (j : ℕ)
+   → (multi_subst (Env.context_terms Γ) f ({j ~> t2} t1))
+     = ({j ~> multi_subst (Env.context_terms Γ) f t2} (multi_subst (Env.context_terms Γ) f t1)) := by
   induction t1
   case bvar k =>
     simp
@@ -1992,7 +1992,7 @@ lemma multi_subst_open_lemma_1 t1 t2 Γ : (f : context_terms Γ → Trm)
       <;> exact hjy
   case fvar y =>
    intro f lcf j
-   by_cases hy : (y ∈ context_terms Γ)
+   by_cases hy : (y ∈ Env.context_terms Γ)
    . simp [opening, multi_subst, hy]
      exact (opening_lc (f ⟨y, hy⟩) _ (lcf y hy) _)
    . simp [opening, multi_subst, hy]
@@ -2007,10 +2007,10 @@ lemma multi_subst_open_lemma_1 t1 t2 Γ : (f : context_terms Γ → Trm)
 
 --special case of previous fact at j=0
 lemma multi_subst_open_lemma_2 Γ t u y T : lc u → y ∉ fv t
-    → (f : context_terms Γ → Trm)
-    → (∀ x (h : x ∈ context_terms Γ), lc (f ⟨x,h⟩))
-    → (multi_subst (context_terms ((y, Bind.bind_typ T) :: Γ)) (add_term Γ f u y T) (open₀ t ($ y)))
-      = (open₀ (multi_subst (context_terms Γ) f t) u) := by
+    → (f : Env.context_terms Γ → Trm)
+    → (∀ x (h : x ∈ Env.context_terms Γ), lc (f ⟨x,h⟩))
+    → (multi_subst (Env.context_terms ((y, Bind.bind_typ T) :: Γ)) (add_term Γ f u y T) (open₀ t ($ y)))
+      = (open₀ (multi_subst (Env.context_terms Γ) f t) u) := by
   intro lcu hy f lcf
   rw [open₀ , multi_subst_open_lemma_1, multi_subst, ← open₀]
   rw [multi_subst_fresh Γ t u y T hy f]
@@ -2024,19 +2024,19 @@ lemma multi_subst_open_lemma_2 Γ t u y T : lc u → y ∉ fv t
 
 --When we open a term, we can instead open the term with a fresh variable and
 --then multi-substitute for that variable.
-lemma multi_subst_open Γ t y : y ∉ context_terms Γ
-    → (f : context_terms Γ → Trm)
-    → (∀ x (h : x ∈ context_terms Γ), lc (f ⟨x,h⟩))
-    → (multi_subst (context_terms Γ) f (open₀ t ($ y)))
-      = (open₀ (multi_subst (context_terms Γ) f t) ($ y)) := by
+lemma multi_subst_open Γ t y : y ∉ Env.context_terms Γ
+    → (f : Env.context_terms Γ → Trm)
+    → (∀ x (h : x ∈ Env.context_terms Γ), lc (f ⟨x,h⟩))
+    → (multi_subst (Env.context_terms Γ) f (open₀ t ($ y)))
+      = (open₀ (multi_subst (Env.context_terms Γ) f t) ($ y)) := by
   intro hy f lcf
   rw [open₀ , multi_subst_open_lemma_1, multi_subst, ← open₀]
   simp [hy]
   apply lcf
 
 --if (x,T) appears in Env Γ, then the Env map sends Γ x to T
-lemma context_type_eq_bind Γ (x : context_terms Γ) T :
-    valid_ctx Γ → binds x T Γ → context_type Γ x = T := by
+lemma context_type_eq_bind Γ (x : Env.context_terms Γ) T :
+    Env.valid_ctx Γ → Env.binds x T Γ → context_type Γ x = T := by
   induction Γ
   case nil =>
     intro _ bnd
@@ -2046,7 +2046,7 @@ lemma context_type_eq_bind Γ (x : context_terms Γ) T :
     cases b with
     | bind_typ S =>
     intro vld bnd
-    simp only [context_type, context_terms]
+    simp only [context_type, Env.context_terms]
     by_cases p : y = ↑x
     . simp [p] at bnd ⊢
       apply bnd
@@ -2061,21 +2061,21 @@ lemma context_type_eq_bind Γ (x : context_terms Γ) T :
 --if a term is locally closed, and there is list of locally closed terms, then
 --substition with these terms is also locally closed.
 lemma multi_subst_lc t Γ : lc t
-    → (f : context_terms Γ → Trm)
-    → (∀ x (h : x ∈ context_terms Γ), lc (f ⟨x,h⟩))
-    → lc ((multi_subst (context_terms Γ) f t)) := by
+    → (f : Env.context_terms Γ → Trm)
+    → (∀ x (h : x ∈ Env.context_terms Γ), lc (f ⟨x,h⟩))
+    → lc ((multi_subst (Env.context_terms Γ) f t)) := by
   intro lct f lcf
   induction lct
   case lc_var y =>
     rw [multi_subst]
-    by_cases hxy : y ∈ context_terms Γ
+    by_cases hxy : y ∈ Env.context_terms Γ
     . simp [if_pos, hxy]
       exact (lcf y hxy)
     . simp [if_neg, hxy]
       exact (lc_var y)
   case lc_abs u T L a hu =>
     simp
-    apply lc_abs _ _ (L ∪ (context_terms Γ))
+    apply lc_abs _ _ (L ∪ (Env.context_terms Γ))
     intro x hx
     simp at hx
     rw [← multi_subst_open Γ u x hx.2 f lcf]
@@ -2390,15 +2390,15 @@ theorem SC_lambda_term A1 A2 t : lc (λ A1,t)
 -- Suppose (x1:A1, x2:A2, ..., xn:An) ⊢ t : A. Then for any strongly computable ui:Ai,
 -- we have ([x1//u1, x2//u2, ..., xn//un] t) is strongly computable.
 lemma SC_subst t A : typing Γ t A
-    → (f : (context_terms Γ) → Trm)
-    → (∀ x (h : x ∈ (context_terms Γ)), (f ⟨x, h⟩) ∈ SC (context_type Γ ⟨x, h⟩))
-    → (multi_subst (context_terms Γ) f t) ∈ SC A := by
+    → (f : (Env.context_terms Γ) → Trm)
+    → (∀ x (h : x ∈ (Env.context_terms Γ)), (f ⟨x, h⟩) ∈ SC (context_type Γ ⟨x, h⟩))
+    → (multi_subst (Env.context_terms Γ) f t) ∈ SC A := by
   intro typt
   induction typt
   case typ_var Δ y T vld bnd =>
     intro f Hf
     simp only [multi_subst]
-    by_cases h : y ∈ context_terms Δ
+    by_cases h : y ∈ Env.context_terms Δ
     . simp [h, ← context_type_eq_bind Δ ⟨y, h⟩ T vld bnd]
       apply (Hf y h)
     . simp [h]
@@ -2412,7 +2412,7 @@ lemma SC_subst t A : typing Γ t A
     intros u1 scu1
     let ⟨x, hx⟩ := pick_fresh u L
     simp at hx
-    have this : (∀ y (s : y ∈ (context_terms ((x, Bind.bind_typ T1) :: Δ))),
+    have this : (∀ y (s : y ∈ (Env.context_terms ((x, Bind.bind_typ T1) :: Δ))),
         ((add_term Δ f u1 x T1) ⟨y, s⟩) ∈ SC (context_type ((x, Bind.bind_typ T1) :: Δ) ⟨y, s⟩)) := by
       intro y s
       by_cases p : y = x
@@ -2429,7 +2429,7 @@ lemma SC_subst t A : typing Γ t A
     intro f Hf
     cases (ih1 f Hf)
     next L R =>
-      apply R (multi_subst (context_terms Δ) f t2)
+      apply R (multi_subst (Env.context_terms Δ) f t2)
       constructor
       . apply multi_subst_lc
         apply (typing_regular _ _ _ typt2)
@@ -2443,14 +2443,14 @@ theorem strong_normalization t T : typing [] t T → SN t := by
   apply CR1 T t
   let ⟨x, hx⟩ := pick_fresh t ∅
   simp at hx
-  let f : context_terms (([(x, Bind.bind_typ T)] : Env)) → Trm := fun _ => ($ x)
-  have this : multi_subst (context_terms (([(x, Bind.bind_typ T)] : Env))) f t = t := by
+  let f : Env.context_terms (([(x, Bind.bind_typ T)] : Env)) → Trm := fun _ => ($ x)
+  have this : multi_subst (Env.context_terms (([(x, Bind.bind_typ T)] : Env))) f t = t := by
     rw [multi_subst_at_singleton]
     rw [subst_fresh _ _ _ hx]
   rw [← this]
   apply SC_subst
   apply typing_weakening [] (([(x, Bind.bind_typ T)] : Env)) _ _ typt
-  apply valid_push _ _ _ (valid_ctx.valid_nil) (by simp)
+  apply valid_push _ _ _ (Env.valid_ctx.valid_nil) (by simp)
   exact (fun y hy => SC_var _ _)
 
 end Trm
@@ -2467,7 +2467,7 @@ theorem typing_unique :
     next _ bnd =>
       cases ty2
       next _ bnd' =>
-        simp [binds] at bnd bnd'
+        simp [Env.binds] at bnd bnd'
         rw [bnd] at bnd'
         simp at bnd'
         exact bnd'
@@ -2492,12 +2492,12 @@ theorem typing_unique :
         exact this
 
 theorem typing_decidable :
-    ∀ t Γ, lc t → valid_ctx Γ →
+    ∀ t Γ, lc t → Env.valid_ctx Γ →
     (∃ T, typing Γ t T) ∨ ¬ (∃ T, typing Γ t T) := by
   intro t Γ lct vld
   induction lct generalizing Γ
   case lc_var x =>
-    match h : (get x Γ) with
+    match h : (Env.get x Γ) with
     | some T =>
         left
         use T
@@ -2509,7 +2509,7 @@ theorem typing_decidable :
         next _ ih =>
           simp [h] at ih
   case lc_abs u T L a ih =>
-    have ⟨x,hx⟩ := pick_fresh u (L ∪ context_terms Γ)
+    have ⟨x,hx⟩ := pick_fresh u (L ∪ Env.context_terms Γ)
     simp at hx
     cases H : (ih x hx.1 ((x, Bind.bind_typ T) :: Γ)
         (valid_push Γ x T vld (not_context_terms_to_not_in_context _ _ hx.2.1)))
@@ -2517,7 +2517,7 @@ theorem typing_decidable :
       rcases pos with ⟨S, p⟩
       left
       use (T -> S)
-      apply (typ_abs (fv u ∪ context_terms Γ) Γ)
+      apply (typ_abs (fv u ∪ Env.context_terms Γ) Γ)
       intro y hy
       simp at hy
       apply typing_rename _ _ _ _ _ _
@@ -2528,7 +2528,7 @@ theorem typing_decidable :
       rintro ⟨S,p⟩
       cases p
       next L' S' h =>
-        have ⟨z,hz⟩ := pick_fresh u (L' ∪ context_terms Γ)
+        have ⟨z,hz⟩ := pick_fresh u (L' ∪ Env.context_terms Γ)
         simp at hz
         apply neg
         use S'
@@ -2579,7 +2579,7 @@ theorem typing_decidable :
         apply neg ⟨_ , ty2⟩
 
 theorem typechecking_decidable t T Γ :
-    lc t → valid_ctx Γ → (typing Γ t T) ∨ ¬(typing Γ t T) := by
+    lc t → Env.valid_ctx Γ → (typing Γ t T) ∨ ¬(typing Γ t T) := by
   intro lct vld
   have this := typing_decidable t Γ lct vld
   cases this
